Test/extern-soundness/ExternalInvariants.dfy
@@ -1,0 +1,214 @@
+
+module ExternalInvariants {
+
+  trait {:termination false} ExternallyValid {
+    ghost const Repr: set<ExternallyValid>
+    predicate Valid() 
+      reads this, Repr 
+      ensures Valid() ==> this in Repr
+      ensures Valid() ==> forall v :: v in Repr ==> v.Repr <= Repr
+      ensures Valid() ==> forall v :: v in Repr && v != this ==> this !in v.Repr
+    
+    // Dummy predicate to avoid "/!\ No terms found to trigger on." warning
+    predicate P() {
+      true
+    }
+
+    // Lemma for re-establishing the external invariant after one object
+    // has changed from valid state to another valid state. Asserts that
+    // all OTHER formally valid objects are still valid based on their
+    // IndependentValidity() lemma.
+    twostate lemma AllStillValid() 
+      requires old(AllValid(set v: ExternallyValid | allocated(v) && v.P()))
+      requires Valid()
+      requires forall o :: o !in Repr ==> unchanged(o)
+      requires forall o :: o in Repr ==> o.Valid()
+      ensures AllValid(set v: ExternallyValid | allocated(v) && v.P())
+    {
+      forall v: ExternallyValid | old(allocated(v)) && v.P() ensures v.Valid() {
+        IndependentValidityInductive(v, Repr);
+      }
+    }
+
+    // Lemma that must be proved for each implementing class. Usually
+    // proves itself with an empty body, provided Valid() is defined
+    // in a compatible way.
+    twostate lemma IndependentValidity()
+      requires old(Valid())
+      requires unchanged(this)
+      requires forall v :: v in Repr && v != this ==> v.Valid()
+      ensures Valid()
+
+    // Slightly silly lemma that might go away if we tweak Dafny's heuristics a bit
+    lemma AllValidMakesMeValid() 
+      requires AllValid(set v: ExternallyValid | allocated(v) && v.P())
+      ensures Valid()
+    {}
+  }
+
+  // This is the "external invariant". It must hold as a precondition and postcondition for
+  // every method that crosses the Dafny/external boundary, either incoming or outgoing.
+  // It assumes that the Dafny heap cannot be changed in any other way.
+  // I have to pass in the set of objects implementing ExternallyValid since I can't pass in
+  // "the Dafny heap".
+  predicate AllValid(vs: set<ExternallyValid>) 
+    reads vs
+    reads set v, o | v in vs && o in v.Repr :: o
+  {
+    forall v :: v in vs ==> v.Valid()
+  }
+
+  twostate lemma IndependentValidityInductive(v: ExternallyValid, changed: set<ExternallyValid>)
+      requires old(AllValid(set v': ExternallyValid | allocated(v') && v'.P()))
+      requires forall o :: o !in changed ==> unchanged(o)
+      requires forall o :: o in changed ==> o.Valid()
+      requires allocated(v)
+      decreases v.Repr
+      ensures v.Valid()
+  {
+    assert old(v.Valid());
+    forall v': ExternallyValid | v' in v.Repr && v' != v && old(allocated(v')) ensures v'.Valid() {
+      IndependentValidityInductive(v', changed);
+    }
+    if v !in changed {
+      v.IndependentValidity();
+    }
+  }
+
+  class NotAtomic extends ExternallyValid {
+
+    var x: int
+    var y: int
+
+    constructor(x: int) 
+      ensures Valid() 
+      ensures fresh(Repr)
+      ensures forall o: ExternallyValid :: allocated(o) && fresh(o) && o.P() ==> o.Valid()
+    {
+      this.x := x;
+      this.y := 2*x;
+      this.Repr := {this};
+    }
+    
+    predicate Valid() 
+      reads this, Repr 
+      ensures Valid() ==> this in Repr
+      ensures Valid() ==> forall v :: v in Repr ==> v.Repr <= Repr
+      ensures Valid() ==> forall v :: v in Repr && v != this ==> this !in v.Repr
+    {
+      && y == 2*x
+      && Repr == {this}
+    }
+    twostate lemma IndependentValidity()
+      requires old(Valid())
+      requires unchanged(this)
+      requires forall v :: v in Repr && v != this ==> v.Valid()
+      ensures Valid()
+    {
+    }
+
+    method Update(x: int) 
+      requires AllValid(set v: ExternallyValid | allocated(v) && v.P())
+      requires Valid() // Should follow automatically since this extends ExternallyValid but ¯\_(ツ)_/¯
+      modifies Repr
+      ensures AllValid(set v: ExternallyValid | allocated(v) && v.P())
+    {
+      this.x := x;
+      
+      // This is not allowed because the external invariant isn't re-established
+      // SomeOtherExternalMethod();
+      
+      // And this fails because `this` is not `ExtValid()` at this point
+      // AllStillValid();
+      
+      this.y := 2*x;
+
+      AllStillValid();
+      SomeOtherExternalMethod();
+    }
+  }
+
+  trait {:extern} ExternalNotAtomic {
+    // TODO-RS: It may be possible to avoid the duplicate definitions of
+    // Valid() and Repr if this trait could extend ExternallyValid itself
+    predicate ExtValid() 
+      reads this, ExtRepr 
+      ensures ExtValid() ==> this in ExtRepr
+    ghost var ExtRepr: set<object>
+
+    method Update(x: int)
+      requires AllValid(set v: ExternallyValid | allocated(v) && v.P())
+      modifies ExtRepr
+      ensures AllValid(set v: ExternallyValid | allocated(v) && v.P())
+  }
+
+  class AsExternalNotAtomic extends ExternalNotAtomic, ExternallyValid {
+    const wrapped: NotAtomic
+    predicate Valid() 
+      reads this, Repr 
+      ensures Valid() ==> this in Repr
+      ensures Valid() ==> forall v :: v in Repr ==> v.Repr <= Repr
+      ensures Valid() ==> forall v :: v in Repr && v != this ==> this !in v.Repr
+      ensures Valid() ==> ExtValid()
+    {
+      && wrapped in Repr
+      && Repr == {this} + wrapped.Repr
+      && wrapped.Valid()
+      && ExtRepr == Repr
+      && ExtValid()
+    }
+
+    predicate ExtValid() 
+      reads this, ExtRepr 
+      ensures ExtValid() ==> this in ExtRepr
+    {
+      && wrapped in ExtRepr
+      && ExtRepr == {this} + wrapped.Repr
+      && wrapped.Valid()
+      && ExtRepr == Repr
+    }
+
+    twostate lemma IndependentValidity()
+      requires old(Valid())
+      requires unchanged(this)
+      requires forall v :: v in Repr && v != this ==> v.Valid()
+      ensures Valid()
+    {}
+
+    constructor(wrapped: NotAtomic) 
+      requires wrapped.Valid() 
+      ensures Valid() 
+      ensures fresh(ExtRepr - wrapped.Repr)
+      ensures forall o: ExternallyValid :: allocated(o) && fresh(o) && o.P() ==> o.Valid()
+    {
+      this.wrapped := wrapped;
+      this.ExtRepr := {this} + wrapped.Repr;
+      this.Repr := ExtRepr;
+    }
+    method Update(x: int) 
+      requires AllValid(set v: ExternallyValid | allocated(v) && v.P())
+      modifies ExtRepr
+      ensures AllValid(set v: ExternallyValid | allocated(v) && v.P())
+    {
+      AllValidMakesMeValid();
+      wrapped.Update(x);
+    }
+  }
+
+  method MakeExternalNotAtomic() returns (res: AsExternalNotAtomic)
+    ensures forall o: ExternallyValid :: allocated(o) && fresh(o) && o.P() ==> o.Valid()
+    ensures res.Valid()
+    ensures fresh(res.ExtRepr)
+  {
+    var internal := new NotAtomic(73);
+    res := new AsExternalNotAtomic(internal);
+  }
+
+  method SomeOtherExternalMethod() 
+    requires AllValid(set v: ExternallyValid | allocated(v) && v.P())
+    ensures AllValid(set v: ExternallyValid | allocated(v) && v.P())
+  {
+    // Do some external stuff
+  }
+}
+
